NuBasicAbstractors.thy
@@ -39,9 +39,9 @@ notation NuRefine (infixl "<where>" 80)
 lemma [simp]: " p \<nuLinkL> N \<nuRefine> P \<nuLinkR> x \<longleftrightarrow> x \<in> P \<and> ( p \<nuLinkL> N \<nuLinkR> x)" unfolding NuRefine_def Refining_ex by auto
 lemma [elim,\<nu>elim]: " x \<ratio> N \<nuRefine> P \<Longrightarrow> (x \<in> P \<Longrightarrow> x \<ratio> N \<Longrightarrow> C) \<Longrightarrow> C" unfolding Inhabited_def by auto
 
-lemma [\<nu>intro]: "\<^bold>i\<^bold>n\<^bold>t\<^bold>r\<^bold>o \<^bold>c\<^bold>a\<^bold>s\<^bold>t N \<longmapsto> x \<tycolon> M \<^bold>w\<^bold>i\<^bold>t\<^bold>h P \<^bold>w\<^bold>h\<^bold>e\<^bold>n Q \<Longrightarrow> \<^bold>i\<^bold>n\<^bold>t\<^bold>r\<^bold>o \<^bold>c\<^bold>a\<^bold>s\<^bold>t N \<longmapsto> x \<tycolon> M <where> S \<^bold>w\<^bold>i\<^bold>t\<^bold>h P \<^bold>w\<^bold>h\<^bold>e\<^bold>n x \<in> S \<and> Q"
+lemma [\<nu>intro]: "\<^bold>i\<^bold>n\<^bold>t\<^bold>r\<^bold>o \<^bold>c\<^bold>a\<^bold>s\<^bold>t x \<tycolon> M \<longmapsto> x \<tycolon> M <where> S \<^bold>w\<^bold>h\<^bold>e\<^bold>n x \<in> S"
   unfolding Intro_def Cast_def by auto
-lemma [\<nu>intro]: "\<^bold>d\<^bold>e\<^bold>s\<^bold>t \<^bold>c\<^bold>a\<^bold>s\<^bold>t x \<tycolon> M \<longmapsto> N \<^bold>w\<^bold>i\<^bold>t\<^bold>h P \<^bold>w\<^bold>h\<^bold>e\<^bold>n Q \<Longrightarrow> \<^bold>d\<^bold>e\<^bold>s\<^bold>t \<^bold>c\<^bold>a\<^bold>s\<^bold>t x \<tycolon> M <where> S \<longmapsto> N \<^bold>w\<^bold>i\<^bold>t\<^bold>h x \<in> S \<and> P \<^bold>w\<^bold>h\<^bold>e\<^bold>n Q"
+lemma [\<nu>intro]: "\<^bold>d\<^bold>e\<^bold>s\<^bold>t \<^bold>c\<^bold>a\<^bold>s\<^bold>t x \<tycolon> M <where> S \<longmapsto> x \<tycolon> M \<^bold>w\<^bold>i\<^bold>t\<^bold>h x \<in> S"
   unfolding Dest_def Cast_def by auto
 lemma refine_\<nu>cast: "\<^bold>p\<^bold>a\<^bold>r\<^bold>a\<^bold>m P \<Longrightarrow> \<^bold>p\<^bold>r\<^bold>e\<^bold>m\<^bold>i\<^bold>s\<^bold>e x \<in> P \<Longrightarrow> \<^bold>c\<^bold>a\<^bold>s\<^bold>t x \<tycolon> N \<longmapsto> x \<tycolon> (N <where> P)" unfolding Cast_def by auto
 
@@ -73,9 +73,9 @@ lemma [elim,\<nu>elim]: " x \<ratio> N <down-lift> g \<Longrightarrow> ( g x \<r
 (* lemma [\<nu>cast_overload E]: " \<^bold>c\<^bold>a\<^bold>s\<^bold>t x \<tycolon> N <down-lift> g \<longmapsto> g x \<tycolon> N" unfolding Cast_def by simp *)
 lemma [\<nu>intro]: "\<^bold>p\<^bold>r\<^bold>e\<^bold>m\<^bold>i\<^bold>s\<^bold>e g x = x' \<Longrightarrow> \<^bold>c\<^bold>a\<^bold>s\<^bold>t x \<tycolon> N <down-lift> g \<longmapsto> x' \<tycolon> N" unfolding Cast_def by auto
 
-lemma [\<nu>intro]: "\<^bold>i\<^bold>n\<^bold>t\<^bold>r\<^bold>o \<^bold>c\<^bold>a\<^bold>s\<^bold>t N \<longmapsto> x \<tycolon> M \<^bold>w\<^bold>i\<^bold>t\<^bold>h P \<^bold>w\<^bold>h\<^bold>e\<^bold>n Q \<Longrightarrow> \<^bold>i\<^bold>n\<^bold>t\<^bold>r\<^bold>o \<^bold>c\<^bold>a\<^bold>s\<^bold>t N \<longmapsto> y \<tycolon> M <down-lift> g \<^bold>w\<^bold>i\<^bold>t\<^bold>h P \<^bold>w\<^bold>h\<^bold>e\<^bold>n (g y = x) \<and> Q"
+lemma [\<nu>intro]: "\<^bold>i\<^bold>n\<^bold>t\<^bold>r\<^bold>o \<^bold>c\<^bold>a\<^bold>s\<^bold>t x \<tycolon> M \<longmapsto> y \<tycolon> M <down-lift> g \<^bold>w\<^bold>h\<^bold>e\<^bold>n (g y = x)"
   unfolding Intro_def Cast_def by auto
-lemma [\<nu>intro]: "\<^bold>d\<^bold>e\<^bold>s\<^bold>t \<^bold>c\<^bold>a\<^bold>s\<^bold>t g y \<tycolon> M \<longmapsto> N \<^bold>w\<^bold>i\<^bold>t\<^bold>h P \<^bold>w\<^bold>h\<^bold>e\<^bold>n Q \<Longrightarrow> \<^bold>d\<^bold>e\<^bold>s\<^bold>t \<^bold>c\<^bold>a\<^bold>s\<^bold>t y \<tycolon> M <down-lift> g \<longmapsto> N \<^bold>w\<^bold>i\<^bold>t\<^bold>h P \<^bold>w\<^bold>h\<^bold>e\<^bold>n Q"
+lemma [\<nu>intro]: "\<^bold>d\<^bold>e\<^bold>s\<^bold>t \<^bold>c\<^bold>a\<^bold>s\<^bold>t y \<tycolon> M <down-lift> g \<longmapsto> g y \<tycolon> M"
   unfolding Dest_def Cast_def by auto
 
 lemma [\<nu>intro]: " \<^bold>c\<^bold>a\<^bold>s\<^bold>t x \<tycolon> N \<longmapsto> y1 \<tycolon> M \<^bold>w\<^bold>i\<^bold>t\<^bold>h P \<Longrightarrow> \<^bold>p\<^bold>r\<^bold>e\<^bold>m\<^bold>i\<^bold>s\<^bold>e y1 = g y  \<Longrightarrow> \<^bold>c\<^bold>a\<^bold>s\<^bold>t x \<tycolon> N \<longmapsto> y \<tycolon> M <down-lift> g" unfolding Cast_def by auto
@@ -100,7 +100,7 @@ lemma [simp]: " p \<nuLinkL> N <up-lift> f \<nuLinkR> x \<longleftrightarrow> (\
   unfolding UpLift_def Refining_ex by auto
 lemma [elim,\<nu>elim]: " x \<ratio> N <up-lift> f \<Longrightarrow> (\<And>y. f y = x \<Longrightarrow> y \<ratio> N \<Longrightarrow> C) \<Longrightarrow> C" unfolding Inhabited_def by auto
 
-lemma [\<nu>intro]: "\<^bold>i\<^bold>n\<^bold>t\<^bold>r\<^bold>o \<^bold>c\<^bold>a\<^bold>s\<^bold>t N \<longmapsto> x \<tycolon> M \<^bold>w\<^bold>i\<^bold>t\<^bold>h P \<^bold>w\<^bold>h\<^bold>e\<^bold>n Q \<Longrightarrow> \<^bold>i\<^bold>n\<^bold>t\<^bold>r\<^bold>o \<^bold>c\<^bold>a\<^bold>s\<^bold>t N \<longmapsto> y \<tycolon> M <up-lift> g \<^bold>w\<^bold>i\<^bold>t\<^bold>h P \<^bold>w\<^bold>h\<^bold>e\<^bold>n (g x = y) \<and> Q"
+lemma [\<nu>intro]: "\<^bold>i\<^bold>n\<^bold>t\<^bold>r\<^bold>o \<^bold>c\<^bold>a\<^bold>s\<^bold>t x \<tycolon> M \<longmapsto> g x \<tycolon> M <up-lift> g"
   unfolding Intro_def Cast_def by auto
 lemma [\<nu>intro]: "(\<And> x.  (g x = y) \<Longrightarrow> \<^bold>d\<^bold>e\<^bold>s\<^bold>t \<^bold>c\<^bold>a\<^bold>s\<^bold>t x \<tycolon> M \<longmapsto> N \<^bold>w\<^bold>i\<^bold>t\<^bold>h P \<^bold>w\<^bold>h\<^bold>e\<^bold>n Q) \<Longrightarrow> \<^bold>d\<^bold>e\<^bold>s\<^bold>t \<^bold>c\<^bold>a\<^bold>s\<^bold>t y \<tycolon> M <up-lift> g \<longmapsto> N \<^bold>w\<^bold>i\<^bold>t\<^bold>h P \<^bold>w\<^bold>h\<^bold>e\<^bold>n Q"
   unfolding Dest_def Cast_def by auto
@@ -183,17 +183,24 @@ lemma [elim,\<nu>elim]: "a \<R_arr_tail> xs \<ratio> Array' N \<Longrightarrow> 
 
 lemma Array'_to_Ref_\<nu>proc[\<nu>intro]:
  "\<^bold>p\<^bold>r\<^bold>e\<^bold>m\<^bold>i\<^bold>s\<^bold>e i < length xs \<Longrightarrow> \<^bold>p\<^bold>r\<^bold>e\<^bold>m\<^bold>i\<^bold>s\<^bold>e (xs ! i) \<noteq> None \<Longrightarrow>
-  \<^bold>c\<^bold>a\<^bold>s\<^bold>t a \<R_arr_tail> xs \<tycolon> Array' N \<longmapsto> a \<R_arr_tail> xs[i := None] \<tycolon> Array' N \<heavy_asterisk> (a ||+ i) \<R_arr_tail> the (xs ! i) \<tycolon> Ref N"
-  unfolding Cast_def apply (cases a) apply auto apply (rule heap_split_by_addr_set[of _  _ "-{a ||+ i}"])
+  \<^bold>d\<^bold>e\<^bold>s\<^bold>t \<^bold>c\<^bold>a\<^bold>s\<^bold>t a \<R_arr_tail> xs \<tycolon> Array' N \<longmapsto> a \<R_arr_tail> xs[i := None] \<tycolon> Array' N \<heavy_asterisk> (a ||+ i) \<R_arr_tail> the (xs ! i) \<tycolon> Ref N"
+  unfolding Dest_def Cast_def apply (cases a) apply auto apply (rule heap_split_by_addr_set[of _  _ "-{a ||+ i}"])
   by (auto simp add: pred_option_def Ball_def nth_list_update)
 
-lemma Array'_dual_Ref_\<nu>proc [\<nu>intro]:
+lemma [\<nu>intro]:
+  "\<^bold>p\<^bold>r\<^bold>e\<^bold>m\<^bold>i\<^bold>s\<^bold>e i < length xs \<Longrightarrow>
+  \<^bold>i\<^bold>n\<^bold>t\<^bold>r\<^bold>o \<^bold>c\<^bold>a\<^bold>s\<^bold>t a \<R_arr_tail> xs[i := None] \<tycolon> Array' N \<heavy_asterisk> (a ||+ i) \<R_arr_tail> y \<tycolon> Ref N \<longmapsto> a \<R_arr_tail> xs[i := Some y] \<tycolon> Array' N"
+  unfolding Intro_def Cast_def apply (cases a) apply (auto simp add: pred_option_def Ball_def)
+  by (metis MemAddrState_add_I1 MemAddrState_add_I2 nth_list_update option.sel)
+
+(* lemma Array'_dual_Ref_\<nu>proc [\<nu>intro]:
  "\<^bold>p\<^bold>r\<^bold>e\<^bold>m\<^bold>i\<^bold>s\<^bold>e i < length xs \<Longrightarrow> \<^bold>p\<^bold>r\<^bold>e\<^bold>m\<^bold>i\<^bold>s\<^bold>e (xs ! i) \<noteq> None \<Longrightarrow>
-  \<^bold>c\<^bold>a\<^bold>s\<^bold>t a \<R_arr_tail> xs \<tycolon> Array' N \<longmapsto> a \<R_arr_tail> xs[i := None] \<tycolon> Array' N \<heavy_asterisk> (a ||+ i) \<R_arr_tail> the (xs ! i) \<tycolon> Ref N
-  \<^bold>d\<^bold>u\<^bold>a\<^bold>l a \<R_arr_tail> xs[i := None] \<tycolon> Array' N \<heavy_asterisk> (a ||+ i) \<R_arr_tail> y \<tycolon> Ref N \<longmapsto> a \<R_arr_tail> xs[i := Some y] \<tycolon> Array' N"
-  unfolding CastDual_def apply (simp add: Array'_to_Ref_\<nu>proc)
+  \<^bold>c\<^bold>a\<^bold>s\<^bold>t a \<R_arr_tail> xs \<tycolon> Array' N \<longmapsto> a \<R_arr_tail> xs[i := None] \<tycolon> Array' N \<heavy_asterisk> \<medium_left_bracket> (a ||+ i) \<R_arr_tail> the (xs ! i) \<tycolon> Ref N \<medium_right_bracket>
+  \<^bold>d\<^bold>u\<^bold>a\<^bold>l a \<R_arr_tail> xs[i := None] \<tycolon> Array' N \<heavy_asterisk> \<medium_left_bracket> (a ||+ i) \<R_arr_tail> y \<tycolon> Ref N \<medium_right_bracket> \<longmapsto> a \<R_arr_tail> xs[i := Some y] \<tycolon> Array' N"
+  unfolding CastDual_def Heap_Cast_Goal_def apply (simp add: Array'_to_Ref_\<nu>proc)
   unfolding Cast_def apply (cases a) apply (auto simp add: pred_option_def Ball_def)
   by (metis MemAddrState_add_I1 MemAddrState_add_I2 nth_list_update option.sel)
+*)
 
 
 subsection \<open>\<nu>-abstraction : Array\<close>
@@ -201,23 +208,24 @@ subsection \<open>\<nu>-abstraction : Array\<close>
 definition Array :: "('a::field, 'b) \<nu> \<Rightarrow> (heap, nat memaddr \<R_arr_tail> 'b list) \<nu>"
   where "Array N = Array' N <down-lift> (map_object id (map Some)) "
 
-lemma [simp]: "heap \<nuLinkL> Array N \<nuLinkR> (base |+ ofs) \<R_arr_tail> xs \<longleftrightarrow>
+(* lemma [simp]: "heap \<nuLinkL> Array N \<nuLinkR> (base |+ ofs) \<R_arr_tail> xs \<longleftrightarrow>
     (ofs + length xs \<le> segment_len base \<and>
     segment_llty base = LLTY('a) \<and>
     (\<forall>i < length xs. heap \<^bold>a\<^bold>t base |+ (ofs + i) \<^bold>i\<^bold>s xs ! i \<tycolon> N)
 )" for N :: "('a::field, 'b) \<nu>"
-  by (auto simp add: lrep_exps Array_def)
+  by (auto simp add: lrep_exps Array_def) *)
   
 lemma [elim,\<nu>elim]: "a \<R_arr_tail> xs \<ratio> Array N \<Longrightarrow> (
     (\<And>i. i < length xs \<Longrightarrow> xs ! i \<ratio> N) \<Longrightarrow> offset_of a + length xs \<le> address_len a \<Longrightarrow> address_llty a = LLTY('a)
   \<Longrightarrow> C) \<Longrightarrow> C"
    for N :: "('a::field, 'b) \<nu>"
   unfolding Inhabited_def[of "\<tort_lbrace>a \<R_arr_tail> xs \<tycolon> Array N\<tort_rbrace>"]
+  unfolding Array_def
   by (cases a) (auto simp add: lrep_exps list_all2_conv_all_nth)
 
 lemma [THEN cast_trans, simplified, \<nu>intro]:
   "\<^bold>c\<^bold>a\<^bold>s\<^bold>t a \<R_arr_tail> xs \<tycolon> Array N \<longmapsto> a \<R_arr_tail> map Some xs \<tycolon> Array' N"
-  unfolding Cast_def by (cases a) auto
+  unfolding Cast_def Array_def by (cases a) auto
 
 definition mapSome :: " 'a list \<Rightarrow> 'a option list " where "mapSome = map Some"
 lemma [simp]: "length (mapSome l) = length l" unfolding mapSome_def by auto
@@ -230,10 +238,16 @@ lemma cast_dual_trans:
     \<Longrightarrow> \<^bold>c\<^bold>a\<^bold>s\<^bold>t A \<longmapsto> C \<^bold>w\<^bold>i\<^bold>t\<^bold>h P1 \<and> P2 \<^bold>d\<^bold>u\<^bold>a\<^bold>l C' \<longmapsto> A' \<^bold>w\<^bold>h\<^bold>e\<^bold>n Q1 \<and> Q2"
   unfolding Cast_def CastDual_def by auto
 
-lemma [THEN cast_dual_trans, \<nu>intro]: 
+lemma [\<nu>intro]: "\<^bold>i\<^bold>n\<^bold>t\<^bold>r\<^bold>o \<^bold>c\<^bold>a\<^bold>s\<^bold>t  a \<R_arr_tail> xs' \<tycolon> Array' N \<longmapsto> a \<R_arr_tail> xs2 \<tycolon> Array N \<^bold>w\<^bold>h\<^bold>e\<^bold>n xs' = mapSome xs2"
+  unfolding Cast_def Intro_def Array_def by (cases a) (auto simp add: pred_option_def Ball_def)
+lemma [\<nu>intro]: "\<^bold>d\<^bold>e\<^bold>s\<^bold>t \<^bold>c\<^bold>a\<^bold>s\<^bold>t a \<R_arr_tail> xs \<tycolon> Array N \<longmapsto> a \<R_arr_tail> mapSome xs \<tycolon> Array' N"
+  unfolding Cast_def Dest_def Array_def by (cases a) (auto simp add: pred_option_def Ball_def)
+
+
+(* lemma [THEN cast_dual_trans, \<nu>intro]: 
   "\<^bold>c\<^bold>a\<^bold>s\<^bold>t a \<R_arr_tail> xs \<tycolon> Array N \<longmapsto> a \<R_arr_tail> mapSome xs \<tycolon> Array' N
   \<^bold>d\<^bold>u\<^bold>a\<^bold>l a \<R_arr_tail> xs' \<tycolon> Array' N \<longmapsto> a \<R_arr_tail> xs2 \<tycolon> Array N \<^bold>w\<^bold>h\<^bold>e\<^bold>n xs' = mapSome xs2"
-  unfolding Cast_def CastDual_def by (cases a) (auto simp add: pred_option_def Ball_def)
+  unfolding Cast_def CastDual_def Array_def by (cases a) (auto simp add: pred_option_def Ball_def) *)
 
 
 subsection \<open>Numbers\<close>
