NuPrime.thy
@@ -312,6 +312,7 @@ definition Different :: " 'a \<Rightarrow> 'a \<Rightarrow> bool " where "Differ
   are not alpha-equivalent. It is useful to break up the self-loop. For example,
   while the introduction rule `cast A \<longmapsto> B \<Longrightarrow> cast B \<longmapsto> C \<Longrightarrow> cast A \<longmapsto> C` causes loop if given `cast A \<longmapsto> A`,
   the rule `cast A \<longmapsto> B \<Longrightarrow> Different A B \<Longrightarrow> cast B \<longmapsto> C \<Longrightarrow> cast A \<longmapsto> C` will not.\<close>
+lemma Different_I: "Different A B" unfolding Different_def ..
 
 subsection \<open>Register and its collection\<close>
 
@@ -747,8 +748,8 @@ theorem cast: "\<^bold>c\<^bold>u\<^bold>r\<^bold>r\<^bold>e\<^bold>n\<^bold>t b
 lemma [\<nu>intro']: "\<^bold>i\<^bold>n\<^bold>t\<^bold>r\<^bold>o \<^bold>c\<^bold>a\<^bold>s\<^bold>t A \<longmapsto> B \<^bold>w\<^bold>i\<^bold>t\<^bold>h P \<Longrightarrow> \<^bold>c\<^bold>a\<^bold>s\<^bold>t A \<longmapsto> B \<^bold>w\<^bold>i\<^bold>t\<^bold>h P" unfolding Intro_def .
 lemma [\<nu>intro']: "\<^bold>d\<^bold>e\<^bold>s\<^bold>t \<^bold>c\<^bold>a\<^bold>s\<^bold>t A \<longmapsto> B \<^bold>w\<^bold>i\<^bold>t\<^bold>h P \<Longrightarrow> \<^bold>c\<^bold>a\<^bold>s\<^bold>t A \<longmapsto> B \<^bold>w\<^bold>i\<^bold>t\<^bold>h P" unfolding Dest_def .
 
-lemma [\<nu>intro'']: "\<^bold>i\<^bold>n\<^bold>t\<^bold>r\<^bold>o \<^bold>c\<^bold>a\<^bold>s\<^bold>t A \<longmapsto> A" unfolding Intro_def using cast_id .
-lemma [\<nu>intro'']: "\<^bold>d\<^bold>e\<^bold>s\<^bold>t \<^bold>c\<^bold>a\<^bold>s\<^bold>t A \<longmapsto> A" unfolding Dest_def using cast_id .
+lemma "\<^bold>i\<^bold>n\<^bold>t\<^bold>r\<^bold>o \<^bold>c\<^bold>a\<^bold>s\<^bold>t A \<longmapsto> A" unfolding Intro_def using cast_id .
+lemma "\<^bold>d\<^bold>e\<^bold>s\<^bold>t \<^bold>c\<^bold>a\<^bold>s\<^bold>t A \<longmapsto> A" unfolding Dest_def using cast_id .
   \<comment> \<open>All intro-cast or dest-cast involved in the reasoner constitute a directed acyclic graph WITH self-loop.
     Note the self-loop has the lowest priority, so that the self-loop only be tried ONCE in the whole reasoning
       (when all other rules cannot be applied), and only longest inference chains (who cannot be extended by
